pred_1_n & bind_1_n => pred & bind

ThoR/Semantics/Semantics.lean
@@ -23,9 +23,9 @@ inductive TyTy : Type 1 where
     | formula : Ty .isTy -- Prop
     | expression : {n : ℕ} → (rel_type : RelType R n) → Ty .isTy-- Rel rel_type
     | function : {n : ℕ} → (t : RelType R n) → Ty .isTy → Ty .isTy -- type1.eval → type2.eval
---    | pred : {n : ℕ} → {t : RelType R n} → Ty (.isPred t) → Ty .isTy
-    | pred_1 : {n : ℕ} → (t : RelType R n) → Ty (.isPred t)
-    | pred_n : {n : ℕ} → (t : RelType R n) → Ty (.isPred t) → Ty (.isPred t)
+    | pred : {n : ℕ} → (t : RelType R n) → Ty (.isPred t)
+    --| pred_1 : {n : ℕ} → (t : RelType R n) → Ty (.isPred t)
+    --| pred_n : {n : ℕ} → (t : RelType R n) → Ty (.isPred t) → Ty (.isPred t)
 
   inductive Marker : Type u where
     | alloy_predicate
@@ -38,9 +38,9 @@ inductive TyTy : Type 1 where
     | .formula => Prop
     | .expression rel_type => Rel rel_type
     | .function dom_rel_type ran => Rel dom_rel_type → ran.eval
-  --  | .pred p => p.eval
-    | .pred_1 dom_rel_type => Rel dom_rel_type → Prop
-    | .pred_n dom_rel_type p' => Rel dom_rel_type → (p'.eval)
+    | .pred t => Rel t →  Prop
+    --| .pred_1 dom_rel_type => Rel dom_rel_type → Prop
+    --| .pred_n dom_rel_type p' => Rel dom_rel_type → (p'.eval)
 
 
 -- variable {R : Type} [TupleSet R] (t : RelType R n)
@@ -57,223 +57,223 @@ inductive TyTy : Type 1 where
     | global_rel_var {n : ℕ} {t : RelType R n} (r : Rel t) (name : String): Term (.expression t)
     | local_rel_var {n : ℕ} {t : RelType R n} (r : Rel t): Term (.expression t)
 
-    -- /- expression constants -/
-    -- --| univ
-    -- --| none
-    -- --| iden
+    /- expression constants -/
+    --| univ
+    --| none
+    --| iden
 
-    -- /- binary expression operators -/
-    -- | union
-    --   {n : ℕ}
-    --   {t1 t2 : RelType R n}
-    --   : Term (.expression t1) →
-    --     Term (.expression t2) →
-    --     Term (.expression (t1 + t2))
+    /- binary expression operators -/
+    | union
+      {n : ℕ}
+      {t1 t2 : RelType R n}
+      : Term (.expression t1) →
+        Term (.expression t2) →
+        Term (.expression (t1 + t2))
 
-    -- | intersect
-    --   {n : ℕ}
-    --   {t1 t2 : RelType R n}
-    --   : Term (.expression t1) →
-    --     Term (.expression t2) →
-    --     Term (.expression (t1 & t2))
+    | intersect
+      {n : ℕ}
+      {t1 t2 : RelType R n}
+      : Term (.expression t1) →
+        Term (.expression t2) →
+        Term (.expression (t1 & t2))
 
-    -- | difference
-    --   {n : ℕ}
-    --   {t1 t2 : RelType R n}
-    --   : Term (.expression t1) →
-    --     Term (.expression t2) →
-    --     Term (.expression (t1 - t2))
+    | difference
+      {n : ℕ}
+      {t1 t2 : RelType R n}
+      : Term (.expression t1) →
+        Term (.expression t2) →
+        Term (.expression (t1 - t2))
 
-    -- | overwrite
-    --   {n : ℕ}
-    --   {t1 t2 : RelType R n}
-    --   : Term (.expression t1) →
-    --     Term (.expression t2) →
-    --     Term (.expression (t1 ++ t2))
+    | overwrite
+      {n : ℕ}
+      {t1 t2 : RelType R n}
+      : Term (.expression t1) →
+        Term (.expression t2) →
+        Term (.expression (t1 ++ t2))
 
-    -- | domain_restriction
-    --   {n : ℕ}
-    --   {t1 : RelType R 1}
-    --   {t2 : RelType R n}
-    --   : Term (.expression t1) →
-    --     Term (.expression t2) →
-    --     Term (.expression (t1 <: t2))
+    | domain_restriction
+      {n : ℕ}
+      {t1 : RelType R 1}
+      {t2 : RelType R n}
+      : Term (.expression t1) →
+        Term (.expression t2) →
+        Term (.expression (t1 <: t2))
 
-    -- | range_restriction
-    --   {n : ℕ}
-    --   {t1 : RelType R n}
-    --   {t2 : RelType R 1}
-    --   : Term (.expression t1) →
-    --     Term (.expression t2) →
-    --     Term (.expression (t1 :> t2))
+    | range_restriction
+      {n : ℕ}
+      {t1 : RelType R n}
+      {t2 : RelType R 1}
+      : Term (.expression t1) →
+        Term (.expression t2) →
+        Term (.expression (t1 :> t2))
 
-    -- | dotjoin
-    --   {n m : ℕ}
-    --   {t1 : RelType R (n+1)}
-    --   {t2 : RelType R (m+2)}
-    --   : Term (.expression t1) →
-    --     Term (.expression t2) →
-    --     Term (.expression (t1 ⋈ t2))
+    | dotjoin
+      {n m : ℕ}
+      {t1 : RelType R (n+1)}
+      {t2 : RelType R (m+2)}
+      : Term (.expression t1) →
+        Term (.expression t2) →
+        Term (.expression (t1 ⋈ t2))
 
-    -- /- unary expression operators -/
-    -- | transclos
-    --   {t : RelType R 2}
-    --   : Term (.expression t) →
-    --     Term (.expression (^ t))
+    /- unary expression operators -/
+    | transclos
+      {t : RelType R 2}
+      : Term (.expression t) →
+        Term (.expression (^ t))
 
-    -- | reflexive_closure
-    --   {t : RelType R 2}
-    --   : Term (.expression t) →
-    --     Term (.expression (* t))
+    | reflexive_closure
+      {t : RelType R 2}
+      : Term (.expression t) →
+        Term (.expression (* t))
 
-    -- | transposition
-    --   {t : RelType R 2}
-    --   : Term (.expression t) →
-    --     Term (.expression (~ t))
+    | transposition
+      {t : RelType R 2}
+      : Term (.expression t) →
+        Term (.expression (~ t))
 
-    -- /- expression if else -/
-    -- | if_then_else
-    --   {n : ℕ}
-    --   {t1 t2 : RelType R n}
-    --   : Term .formula →
-    --     Term (.expression t1) →
-    --     Term (.expression t2) →
-    --     Term (.expression (RelType.ifThenElse t1 t2))
+    /- expression if else -/
+    | if_then_else
+      {n : ℕ}
+      {t1 t2 : RelType R n}
+      : Term .formula →
+        Term (.expression t1) →
+        Term (.expression t2) →
+        Term (.expression (RelType.ifThenElse t1 t2))
 
-    -- /- function call from expression ? -/
-    -- --| call -- skip ?
+    /- function call from expression ? -/
+    --| call -- skip ?
 
-    -- /--bracket definition-/
-    -- | bracket : Term ty → Term ty
+    /--bracket definition-/
+    | bracket : Term ty → Term ty
 
-    -- /--predicate definition-/
-    -- | pred_def (name : String) : Term ty → Term ty
+    /--predicate definition-/
+    | pred_def (name : String) : Term ty → Term ty
 
-    -- /--function definition-/
-    -- | fun_def (name : String) : Term ty → Term ty
-    -- -- | marker : Marker → Term ty → Term ty
-    -- -- | name : String → Term ty → Term ty
+    /--function definition-/
+    | fun_def (name : String) : Term ty → Term ty
+    -- | marker : Marker → Term ty → Term ty
+    -- | name : String → Term ty → Term ty
 
-    -- /- algebra expression number -/
-    -- | number (z : ℤ) : Term .number -- may have to be from N
+    /- algebra expression number -/
+    | number (z : ℤ) : Term .number -- may have to be from N
 
-    -- /- algebra expression unary operation -/
-    -- | negation : Term .number → Term .number
+    /- algebra expression unary operation -/
+    | negation : Term .number → Term .number
 
-    -- /- algebra expression binary operation -/
-    -- | add
-    --   : Term .number →
-    --   Term .number →
-    --   Term .number
+    /- algebra expression binary operation -/
+    | add
+      : Term .number →
+      Term .number →
+      Term .number
 
-    -- | sub
-    --   : Term .number →
-    --   Term .number →
-    --   Term .number
+    | sub
+      : Term .number →
+      Term .number →
+      Term .number
 
-    -- | mul
-    --   : Term .number →
-    --     Term .number →
-    --     Term .number
+    | mul
+      : Term .number →
+        Term .number →
+        Term .number
 
-    -- | div
-    --   : Term .number →
-    --     Term .number →
-    --     Term .number
+    | div
+      : Term .number →
+        Term .number →
+        Term .number
 
-    -- | rem
-    --   : Term .number →
-    --     Term .number →
-    --     Term .number
+    | rem
+      : Term .number →
+        Term .number →
+        Term .number
 
-    -- /- algebra expression card operation (rel operation)-/
-    -- | card
-    --   {n : ℕ}
-    --   {t : RelType R n}
-    --   : Term (.expression t) →
-    --     Term .number
+    /- algebra expression card operation (rel operation)-/
+    | card
+      {n : ℕ}
+      {t : RelType R n}
+      : Term (.expression t) →
+        Term .number
 
-    -- /- formula unary rel bool operator-/
-    -- | no
-    --   {n : ℕ}
-    --   {t : RelType R n}
-    --   : Term (.expression t) →
-    --     Term .formula
+    /- formula unary rel bool operator-/
+    | no
+      {n : ℕ}
+      {t : RelType R n}
+      : Term (.expression t) →
+        Term .formula
 
-    -- | one
-    --   {n : ℕ}
-    --   {t : RelType R n}
-    --   : Term (.expression t) →
-    --     Term .formula
+    | one
+      {n : ℕ}
+      {t : RelType R n}
+      : Term (.expression t) →
+        Term .formula
 
-    -- | lone
-    --   {n : ℕ}
-    --   {t : RelType R n}
-    --   : Term (.expression t) →
-    --     Term .formula
+    | lone
+      {n : ℕ}
+      {t : RelType R n}
+      : Term (.expression t) →
+        Term .formula
 
-    -- | some
-    --   {n : ℕ}
-    --   {t : RelType R n}
-    --   : Term (.expression t) →
-    --     Term .formula
+    | some
+      {n : ℕ}
+      {t : RelType R n}
+      : Term (.expression t) →
+        Term .formula
 
-    -- /- formula unary logic operator -/
-    -- | not : Term .formula → Term .formula
+    /- formula unary logic operator -/
+    | not : Term .formula → Term .formula
 
-    -- /- formula binary logic operator -/
-    -- | or
-    --   : Term .formula →
-    --     Term .formula →
-    --     Term .formula
+    /- formula binary logic operator -/
+    | or
+      : Term .formula →
+        Term .formula →
+        Term .formula
 
-    -- | and
-    --   : Term .formula →
-    --     Term .formula →
-    --     Term .formula
+    | and
+      : Term .formula →
+        Term .formula →
+        Term .formula
 
-    -- | implication
-    --   : Term .formula →
-    --     Term .formula →
-    --     Term .formula
+    | implication
+      : Term .formula →
+        Term .formula →
+        Term .formula
 
-    -- | equivalent
-    --   : Term .formula →
-    --     Term .formula →
-    --     Term .formula
+    | equivalent
+      : Term .formula →
+        Term .formula →
+        Term .formula
 
-    -- /- formula if else-/
-    -- | f_if_then_else
-    --   : Term .formula →
-    --     Term .formula →
-    --     Term .formula →
-    --     Term .formula
+    /- formula if else-/
+    | f_if_then_else
+      : Term .formula →
+        Term .formula →
+        Term .formula →
+        Term .formula
 
-    -- /- formula algebraic comparison operator -/
-    -- | algebraic_leq
-    --   : Term .number →
-    --     Term .number →
-    --     Term .formula
+    /- formula algebraic comparison operator -/
+    | algebraic_leq
+      : Term .number →
+        Term .number →
+        Term .formula
 
-    -- | algebraic_geq
-    --   : Term .number →
-    --     Term .number →
-    --     Term .formula
+    | algebraic_geq
+      : Term .number →
+        Term .number →
+        Term .formula
 
-    -- | algebraic_eq
-    --   : Term .number →
-    --     Term .number →
-    --     Term .formula
+    | algebraic_eq
+      : Term .number →
+        Term .number →
+        Term .formula
 
-    -- | algebraic_lt
-    --   : Term .number →
-    --     Term .number →
-    --     Term .formula
+    | algebraic_lt
+      : Term .number →
+        Term .number →
+        Term .formula
 
-    -- | algebraic_gt
-    --   : Term .number →
-    --     Term .number →
-    --     Term .formula
+    | algebraic_gt
+      : Term .number →
+        Term .number →
+        Term .formula
 
     /- formula relation comparison operation -/
     | in
@@ -283,74 +283,91 @@ inductive TyTy : Type 1 where
         (expression2 : Term (.expression t2)) →
         Term .formula
 
-    -- | eq
-    --   {n : ℕ}
-    --   {t1 t2 : RelType R n}
-    --   : (expression1 : Term (.expression t1)) →
-    --     (expression2 : Term (.expression t2)) →
-    --     Term .formula
+    | eq
+      {n : ℕ}
+      {t1 t2 : RelType R n}
+      : (expression1 : Term (.expression t1)) →
+        (expression2 : Term (.expression t2)) →
+        Term .formula
 
-    -- | neq
-    --   {n : ℕ}
-    --   {t1 t2 : RelType R n}
-    --   : (expression1 : Term (.expression t1)) →
-    --     (expression2 : Term (.expression t2)) →
-    --     Term .formula
+    | neq
+      {n : ℕ}
+      {t1 t2 : RelType R n}
+      : (expression1 : Term (.expression t1)) →
+        (expression2 : Term (.expression t2)) →
+        Term .formula
 
-    -- /- function abstraction -/
-    -- | lam (t : RelType R n)
-    --   : (Rel t → Term ran) →
-    --     Term (.function t ran)
+    /- function abstraction -/
+    | lam (t : RelType R n)
+      : (Rel t → Term ran) →
+        Term (.function t ran)
 
-    -- /- function application / application of argument to call ? -/
-    -- | app
-    --   : Term (.function t ran) →
-    --     Term (.expression t) →
-    --     Term ran
+    /- function application / application of argument to call ? -/
+    | app
+      : Term (.function t ran) →
+        Term (.expression t) →
+        Term ran
 
     | q_group
       : Shared.quant →
         Term .formula →
         Term .formula
 
-    | pred_1 {n : ℕ} {t : RelType R n}
-      : (Rel t → Term .formula) →
-        Term (Ty.pred_1 t)
-    | pred_n {n : ℕ} {t : RelType R n} {ran : Ty (.isPred t)}
-      : (Rel t → Term ran) →
-        Term (Ty.pred_n t ran)
+    -- | pred_1 {n : ℕ} {t : RelType R n}
+    --   : (Rel t → Term .formula) →
+    --     Term (Ty.pred_1 t)
+    -- | pred_n {n : ℕ} {t : RelType R n} {ran : Ty (.isPred t)}
+    --   : (Rel t → Term ran) →
+    --     Term (Ty.pred_n t ran)
 
-    | bind_1 {t : RelType R n}
+    | pred {n : ℕ} {t : RelType R n}
+      : (Rel t → Term .formula) →
+        Term (.pred t)
+
+    -- | bind_1 {t : RelType R n}
+    --   : (m : Shared.quant) →
+    --     (unary_pred : Term (Ty.pred_1 t)) →
+    --     (parameter : Term (.expression t)) →
+    --     Term .formula
+    -- | bind_n {t : RelType R n} {ran : Ty (.isPred t)}
+    --   : (m : Shared.quant) →
+    --     (nary_pred : Term (Ty.pred_n t ran)) →
+    --     (parameter : Term (.expression t)) →
+    --     Term ran
+
+    | bind {t : RelType R n}
       : (m : Shared.quant) →
-        (unary_pred : Term (Ty.pred_1 t)) →
-        (parameter : Term (.expression t)) →
+        (pred : Term (.pred t)) →
         Term .formula
-    | bind_n {t : RelType R n} {ran : Ty (.isPred t)}
-      : (m : Shared.quant) →
-        (nary_pred : Term (Ty.pred_n t ran)) →
-        (parameter : Term (.expression t)) →
-        Term ran
 
 
 variable {R : Type} [TupleSet R] (t : RelType R n)
-#check Term.pred_1 (λ (r : Rel t) => Term.in
+#check Term.pred (λ (r : Rel t) => Term.in
               (expression1 := Term.local_rel_var r)
               (expression2 := Term.local_rel_var r) )
-#check Term.pred_n (
-    λ (q : Rel t) => Term.pred_1 (
-      λ (r : Rel t) =>
-        Term.in
-          (expression1 := Term.local_rel_var q)
-          (expression2 := Term.local_rel_var r)
+#check Term.pred (
+    λ (q : Rel t) =>
+    Term.bind
+      (Shared.quant.all)
+      (Term.pred (
+        λ (r : Rel t) =>
+          Term.in
+            (expression1 := Term.local_rel_var q)
+            (expression2 := Term.local_rel_var r)
+        )
       )
 )
 
-def p1 := Term.pred_n (
-    λ (q : Rel t) => Term.pred_1 (
+def p1 := Term.pred (
+    λ (q : Rel t) =>
+    Term.bind
+      (Shared.quant.all)
+      (Term.pred (
       λ (r : Rel t) =>
         Term.in
           (expression1 := Term.local_rel_var q)
           (expression2 := Term.local_rel_var r)
+        )
       )
 )
 
@@ -360,13 +377,17 @@ def p1 := Term.pred_n (
 -- set_option diagnostics true
 -- set_option diagnostics.threshold 0
 
-example : p1 t = Term.pred_n (
-    λ (q : Rel t) => Term.pred_1 (
-      λ (r : Rel t) =>
-        Term.in
-          (expression1 := Term.local_rel_var q)
-          (expression2 := Term.local_rel_var r)
-      )
+example : p1 t = Term.pred (
+    λ (q : Rel t) =>
+      Term.bind
+        (Shared.quant.all)
+        (Term.pred
+          (λ (r : Rel t) =>
+              Term.in
+                (expression1 := Term.local_rel_var q)
+                (expression2 := Term.local_rel_var r)
+          )
+        )
 ) := by
   sorry
 
@@ -385,119 +406,122 @@ example : p1 t = Term.pred_n (
       | .local_rel_var r => r
 
       /- binary expression operators -/
-      --| .intersect r1 r2 => (r1.eval) & (r2.eval)
-      --| .union r1 r2 => HAdd.hAdd (r1.eval) (r2.eval)
-      --| .difference r1 r2 => (r1.eval) - (r2.eval)
-      --| .overwrite r1 r2 => (r1.eval) ++ (r2.eval)
-      --| .domain_restriction r1 r2 => (r1.eval) <: (r2.eval)
-      --| .range_restriction r1 r2 => (r1.eval) :> (r2.eval)
-      --| .dotjoin r1 r2 => (r1.eval) ⋈ (r2.eval)
+      | .intersect r1 r2 => (r1.eval) & (r2.eval)
+      | .union r1 r2 => HAdd.hAdd (r1.eval) (r2.eval)
+      | .difference r1 r2 => (r1.eval) - (r2.eval)
+      | .overwrite r1 r2 => (r1.eval) ++ (r2.eval)
+      | .domain_restriction r1 r2 => (r1.eval) <: (r2.eval)
+      | .range_restriction r1 r2 => (r1.eval) :> (r2.eval)
+      | .dotjoin r1 r2 => (r1.eval) ⋈ (r2.eval)
 
       /- unary expression operators -/
-      --| .transclos r => ^ (r.eval)
-      --| .reflexive_closure  r => * (r.eval)
-      --| .transposition r => ~ (r.eval)
+      | .transclos r => ^ (r.eval)
+      | .reflexive_closure  r => * (r.eval)
+      | .transposition r => ~ (r.eval)
 
       /- expression if else -/
-      --| .if_then_else f r1 r2 => HIfThenElse.hIfThenElse (f.eval) (r1.eval) (r2.eval)
+      | .if_then_else f r1 r2 => HIfThenElse.hIfThenElse (f.eval) (r1.eval) (r2.eval)
 
-      --| .bracket t => t.eval
-      --| .pred_def _ t => t.eval
-      --| .fun_def _ t => t.eval
+      | .bracket t => t.eval
+      | .pred_def _ t => t.eval
+      | .fun_def _ t => t.eval
       -- | .marker _ t => t.eval
       -- | .name _ t => t.eval
 
-      --| @Term.lam R _ _ _ t f => λ (x : Rel t) => (f x).eval
-      --| .app f r => f.eval r.eval
+      | @Term.lam R _ _ _ t f => λ (x : Rel t) => (f x).eval
+      | .app f r => f.eval r.eval
 
       | .q_group m p => p.eval
 
-      | .pred_1 f =>
-        let result := λ x => (f x).eval
-        result
+      -- | .pred_1 f =>
+      --   let result := λ x => (f x).eval
+      --   result
 
-      | @Term.pred_n R _ n t ran f =>
-        let result := ( λ x => (f x).eval : Rel t → ran.eval )
-        result
+      -- | @Term.pred_n R _ n t ran f =>
+      --   let result := ( λ x => (f x).eval : Rel t → ran.eval )
+      --   result
 
-      | @Term.bind_1 R _ _ t m f parameter =>
-        let function := f.eval
-        let param := parameter.eval -- unused currently ?
-        let result := ∀ x, function x
-        result
+      | .pred f => fun x => (f x).eval
 
-      | @Term.bind_n R _ arity relType range quantifier term parameter =>
-        let test1 := @Term.eval R _ tt ty t
-        let test2 := parameter.eval
+      -- | @Term.bind_1 R _ _ t m f parameter =>
+      --   let function := f.eval
+      --   let param := parameter.eval -- unused currently ?
+      --   let result := ∀ x, function x
+      --   result
 
-        let function := term.eval
-        let param := parameter.eval
+      -- | @Term.bind_n R _ arity relType range quantifier term parameter =>
+      --   let test1 := @Term.eval R _ tt ty t
+      --   let test2 := parameter.eval
 
-        /-possible problem? : cant use ∀ outside of prop ?-/
-        let result := (function param : range.eval)
-        result
+      --   let function := term.eval
+      --   let param := parameter.eval
 
+      --   /-possible problem? : cant use ∀ outside of prop ?-/
+      --   let result := (function param : range.eval)
+      --   result
 
-      --| .number z => z
+      | .bind m f => ∀ x, f.eval x
+
+      | .number z => z
 
       /- algebra expression unary operation -/
-      --| .negation z => - (z.eval)
+      | .negation z => - (z.eval)
 
       /- algebra expression binary operation -/
-      --| .add z1 z2 => (z1.eval) + (z2.eval)
-      --| .sub z1 z2 => (z1.eval) - (z2.eval)
-      --| .div z1 z2 => (z1.eval) / (z2.eval)
-      --| .mul z1 z2 => (z1.eval) * (z2.eval)
-      --| .rem z1 z2 => (z1.eval) % (z2.eval)
+      | .add z1 z2 => (z1.eval) + (z2.eval)
+      | .sub z1 z2 => (z1.eval) - (z2.eval)
+      | .div z1 z2 => (z1.eval) / (z2.eval)
+      | .mul z1 z2 => (z1.eval) * (z2.eval)
+      | .rem z1 z2 => (z1.eval) % (z2.eval)
 
       /- algebra expression card operation (rel operation)-/
-      --| .card r => Card.card (r.eval)
+      | .card r => Card.card (r.eval)
 
       /- formula unary rel bool operator-/
-      -- | .no r => SetMultPredicates.no (r.eval)
-      -- | .one r => SetMultPredicates.one (r.eval)
-      -- | .lone r => SetMultPredicates.lone (r.eval)
-      -- | .some r => SetMultPredicates.some (r.eval)
+      | .no r => SetMultPredicates.no (r.eval)
+      | .one r => SetMultPredicates.one (r.eval)
+      | .lone r => SetMultPredicates.lone (r.eval)
+      | .some r => SetMultPredicates.some (r.eval)
 
       /- formula unary logic operator -/
-      -- | .not f => ¬ (f.eval)
+      | .not f => ¬ (f.eval)
 
       /- formula binary logic operator -/
-      -- | .or f1 f2 => (f1.eval) ∨ (f2.eval)
-      -- | .and f1 f2 => (f1.eval) ∧ (f2.eval)
-      -- | .implication f1 f2 => (f1.eval) → (f2.eval)
-      -- | .equivalent f1 f2 => (f1.eval) = (f2.eval)
+      | .or f1 f2 => (f1.eval) ∨ (f2.eval)
+      | .and f1 f2 => (f1.eval) ∧ (f2.eval)
+      | .implication f1 f2 => (f1.eval) → (f2.eval)
+      | .equivalent f1 f2 => (f1.eval) = (f2.eval)
 
       /- formula if else -/
-      -- | .f_if_then_else f1 f2 f3 =>
-      --   ((f1.eval) -> (f2.eval)) ∧ (¬ (f1.eval) → (f2.eval))
+      | .f_if_then_else f1 f2 f3 =>
+        ((f1.eval) -> (f2.eval)) ∧ (¬ (f1.eval) → (f2.eval))
 
       /- formula algebraic comparison operator -/
-      -- | .algebraic_leq z1 z2 => (z1.eval) <= (z2.eval)
-      -- | .algebraic_geq z1 z2 => (z1.eval) >= (z2.eval)
-      -- | .algebraic_lt z1 z2 => (z1.eval) < (z2.eval)
-      -- | .algebraic_gt z1 z2 => (z1.eval) > (z2.eval)
-      -- | .algebraic_eq z1 z2 => (z1.eval) = (z2.eval)
+      | .algebraic_leq z1 z2 => (z1.eval) <= (z2.eval)
+      | .algebraic_geq z1 z2 => (z1.eval) >= (z2.eval)
+      | .algebraic_lt z1 z2 => (z1.eval) < (z2.eval)
+      | .algebraic_gt z1 z2 => (z1.eval) > (z2.eval)
+      | .algebraic_eq z1 z2 => (z1.eval) = (z2.eval)
 
       /- formula relation comparison operation -/
       | .in r1 r2 => (r1.eval) ⊂ (r2.eval)
-      -- | .eq r1 r2 => (r1.eval) ≡ (r2.eval)
-      -- | .neq r1 r2 => (r1.eval) ≢  (r2.eval)
+      | .eq r1 r2 => (r1.eval) ≡ (r2.eval)
+      | .neq r1 r2 => (r1.eval) ≢  (r2.eval)
 
       -- | q_group {t : RelType R n} {ran : Ty (.isPred t)}
       --     : Shared.quant →
       --       Term ran →
       --       Term .formula
 
---   instance {R : Type} [TupleSet R] {ty : @Ty R _} (t : @Term R _ ty):
---     CoeDep (@Term R _ ty) t ty.eval where
---       coe := t.eval
+  -- instance {R : Type} [TupleSet R] {ty : @Ty R _} (t : @Term R _ ty):
+  --   CoeDep (@Term R _ ty) t ty.eval where
+  --     coe := t.eval
 
---   instance {R : Type} [TupleSet R] {n : ℕ} (t : @Term R _ (Ty.type n)):
---     CoeDep _ t Type where
---       coe := Rel t.eval
+  -- instance {R : Type} [TupleSet R] {n : ℕ} (t : @Term R _ (Ty.type n)):
+  --   CoeDep _ t Type where
+  --     coe := Rel t.eval
 
--- end ThoR.Semantics
+end ThoR.Semantics
 
 -- /-
 -- all disj x, y, z : r | ...
